Fix boolean decoder vst spec

src/Lib/Lib.v
@@ -31,6 +31,8 @@ Definition primitive_encoder td ls : errW1 asn_enc_rval :=
 
 Definition ZeroChar := Byte.repr 48.
 
-Definition byte_of_bool (b : byte) := if (b == default_byte)%byte 
+Definition bool_of_byte (b : byte) := if (b == default_byte)%byte 
                                       then false
                                       else true.
+
+Definition bool_to_byte (b : bool) := if b then (Byte.repr 255) else (default_byte).
